[SoE] Add 'p' as the "next prime" to the Sieve
Also include the constraints 'hppos', 'hpprime', and 'hpnext'

Previously these were all passed to each theorem separately. Now
they're included in the 'Sieve' structure itself.

FormalVerifyMisc/CodeChef/Template/Primes.lean
@@ -13,8 +13,12 @@ set_option linter.style.commandStart false
 def SIEVE_SIZE : ℕ := 1000001
 
 structure Sieve (L : ℕ) where
+  -- The sieve - with non-zero values indicating divisors
   divs : Array Int32
+  -- The list of primes found thus far
   primes : Array Int32
+  -- The next prime to be added to the sieve
+  p : Int32
   -- The size of 'divs' is given by 'L'
   hsize : divs.size = L
   -- The length of the sieve has an upper bound
@@ -23,15 +27,22 @@ structure Sieve (L : ℕ) where
   -- The entries in the sieve are non-negative
   hdivsnn : ∀ x ∈ divs, 0 ≤ x
   -- The values in 'primes' are all positive
-  hprimespos : ∀ p ∈ primes, 0 < p
-  -- For every value 'p' in 'primes', every multiple of 'p' is marked in 'divs'
-  hmarked : ∀ p ∈ primes, ∀ i, (0 < i) → (ilt : i < divs.size) →
-    p.toInt ∣ (i : ℤ) → divs[i] ≠ 0
+  hprimespos : ∀ q ∈ primes, 0 < q
+  -- 'p' is positive
+  hppos : 0 < p
+  -- The absolute value of 'p' is prime
+  hpprime : Nat.Prime p.toInt.natAbs
+  -- Any prime less than 'p' is already in 'primes'
+  hpnext : ∀ q, Nat.Prime q → (q : ℤ) < p.toInt →
+    (q : ℤ) ∈ (Array.map Int32.toInt primes)
+  -- For every value 'q' in 'primes', every multiple of 'q' is marked in 'divs'
+  hmarked : ∀ q ∈ primes, ∀ i, (0 < i) → (ilt : i < divs.size) →
+    q.toInt ∣ (i : ℤ) → divs[i] ≠ 0
   -- A natural number is in 'primes' if-and-only-if it is a prime
   -- less than or equal to the last value in 'primes'
-  hpmem_iff : (hnnil : primes ≠ #[]) → ∀ p : ℕ,
-    ((p : ℤ) ∈ (Array.map Int32.toInt primes) ↔
-     (p : ℤ) ≤ (primes.back (Array.size_pos_iff.mpr hnnil)).toInt ∧ Nat.Prime p)
+  hpmem_iff : (hnnil : primes ≠ #[]) → ∀ q : ℕ,
+    ((q : ℤ) ∈ (Array.map Int32.toInt primes) ↔
+     (q : ℤ) ≤ (primes.back (Array.size_pos_iff.mpr hnnil)).toInt ∧ Nat.Prime q)
   -- If an entry in the sieve is non-zero, its value corresponds to the smallest
   -- divisor of its index greater than 1
   hdivs_dvd : ∀ i, (ilt : i < divs.size) → divs[i]'(ilt) ≠ 0 →
@@ -42,6 +53,7 @@ structure Sieve (L : ℕ) where
 def init_sieve : Sieve SIEVE_SIZE where
   divs := Array.replicate SIEVE_SIZE 0
   primes := #[]
+  p := 2
   hsize := Array.size_replicate
   hLlt := by
     unfold SIEVE_SIZE;
@@ -51,6 +63,13 @@ def init_sieve : Sieve SIEVE_SIZE where
     rw [(Array.mem_replicate.mp xmem).2]; rfl
   hprimespos :=
     fun _ hmem ↦ False.elim (Array.not_mem_empty _ hmem)
+  hppos := rfl
+  hpprime := by
+    simp; norm_num
+  hpnext := by
+    intro q qprime qlt
+    absurd qlt; simp
+    exact Nat.Prime.two_le qprime
   hmarked := by
     intro _ pmem
     exact False.elim (Array.not_mem_empty _ pmem)
@@ -62,16 +81,14 @@ def init_sieve : Sieve SIEVE_SIZE where
     · intro y lty ydvd; simp
 
 -- Update the sieve to indicate that 'p' is the smallest divisor of 'n'
-def mark_sieve {L : ℕ} (S : Sieve L) (p n : Int32)
-  (hppos : 0 < p) (hnpos : 0 < n)
+def mark_sieve {L : ℕ} (S : Sieve L) (n : Int32)
+  (hnpos : 0 < n)
   (nlt : n.toInt.natAbs < S.divs.size)
-  (hprime : Nat.Prime p.toInt.natAbs)
-  (hnextp : ∀ q, Nat.Prime q → (q : ℤ) < p.toInt →
-    (q : ℤ) ∈ (Array.map Int32.toInt S.primes))
-  (hdvd : p.toInt ∣ n.toInt) : Sieve L where
+  (hdvd : S.p.toInt ∣ n.toInt) : Sieve L where
   divs := if S.divs[n.toInt.natAbs] ≠ 0 then S.divs
-    else S.divs.set n.toInt.natAbs p nlt
+    else S.divs.set n.toInt.natAbs S.p nlt
   primes := S.primes
+  p := S.p
   hsize := by
     split_ifs with h
     · exact S.hsize
@@ -86,9 +103,12 @@ def mark_sieve {L : ℕ} (S : Sieve L) (p n : Int32)
     · intro xmem
       rcases Array.mem_or_eq_of_mem_set xmem with lhs | rhs
       · exact S.hdivsnn x lhs
-      · rw [← rhs] at hppos
-        exact Int32.le_of_lt hppos
+      · rw [rhs]
+        exact Int32.le_of_lt S.hppos
   hprimespos := S.hprimespos
+  hppos := S.hppos
+  hpprime := S.hpprime
+  hpnext := S.hpnext
   hmarked := by
     intro q qmem i ipos
     split_ifs with h
@@ -97,7 +117,9 @@ def mark_sieve {L : ℕ} (S : Sieve L) (p n : Int32)
     · intro ilt qdvd
       rw [Array.getElem_set nlt ilt]
       split_ifs with h'
-      · contrapose! hppos; subst hppos; simp
+      · intro h
+        absurd S.hppos
+        rw [h]; simp
       · rw [Array.size_set nlt] at ilt
         exact S.hmarked q qmem i ipos ilt qdvd
   hpmem_iff := S.hpmem_iff
@@ -126,7 +148,7 @@ def mark_sieve {L : ℕ} (S : Sieve L) (p n : Int32)
           apply int32_toInt_ne_zero_of_ne_zero
           exact (Int32.ne_of_lt hnpos).symm
         have qley : q ≤ y := Nat.le_of_dvd (lt_trans (by norm_num) lty) qdvdy
-        have qmem := hnextp q qprime (lt_of_le_of_lt (Int.ofNat_le_ofNat_of_le qley) h)
+        have qmem := S.hpnext q qprime (lt_of_le_of_lt (Int.ofNat_le_ofNat_of_le qley) h)
         rcases Array.exists_of_mem_map qmem with ⟨m, mmem, hmq⟩
         apply S.hmarked m mmem _ nabspos nlt
         rw [hmq]
@@ -135,35 +157,32 @@ def mark_sieve {L : ℕ} (S : Sieve L) (p n : Int32)
         rw [Array.size_set nlt] at ilt
         exact S.hdivs_dvd i ilt hinz
 
-@[simp] theorem mark_sieve_divs_size {L : ℕ} (S : Sieve L) (p n : Int32)
-  (hppos : 0 < p) (hnpos : 0 < n)
+@[simp] theorem mark_sieve_divs_size {L : ℕ} (S : Sieve L) (n : Int32)
+  (hnpos : 0 < n)
   (nlt : n.toInt.natAbs < S.divs.size)
-  (hprime : Nat.Prime p.toInt.natAbs)
-  (hnextp : ∀ q, Nat.Prime q → (q : ℤ) < p.toInt →
-    (q : ℤ) ∈ (Array.map Int32.toInt S.primes))
-  (hdvd : p.toInt ∣ n.toInt) :
-  (mark_sieve S p n hppos hnpos nlt hprime hnextp hdvd).divs.size = S.divs.size := by
+  (hdvd : S.p.toInt ∣ n.toInt) :
+  (mark_sieve S n hnpos nlt hdvd).divs.size = S.divs.size := by
   rw [Sieve.hsize, Sieve.hsize]
 
-@[simp] theorem mark_sieve_primes {L : ℕ} (S : Sieve L) (p n : Int32)
-  (hppos : 0 < p) (hnpos : 0 < n)
+@[simp] theorem mark_sieve_primes {L : ℕ} (S : Sieve L) (n : Int32)
+  (hnpos : 0 < n)
   (nlt : n.toInt.natAbs < S.divs.size)
-  (hprime : Nat.Prime p.toInt.natAbs)
-  (hnextp : ∀ q, Nat.Prime q → (q : ℤ) < p.toInt →
-    (q : ℤ) ∈ (Array.map Int32.toInt S.primes))
-  (hdvd : p.toInt ∣ n.toInt) :
-  (mark_sieve S p n hppos hnpos nlt hprime hnextp hdvd).primes = S.primes := rfl
+  (hdvd : S.p.toInt ∣ n.toInt) :
+  (mark_sieve S n hnpos nlt hdvd).primes = S.primes := rfl
+
+@[simp] theorem mark_sieve_next_prime {L : ℕ} (S : Sieve L) (n : Int32)
+  (hnpos : 0 < n)
+  (nlt : n.toInt.natAbs < S.divs.size)
+  (hdvd : S.p.toInt ∣ n.toInt) :
+  (mark_sieve S n hnpos nlt hdvd).p = S.p := rfl
 
 -- Every cell marked in 'S' is also marked in 'mark_sieve S'
-theorem mark_sieve_marked_of_marked {L : ℕ} (S : Sieve L) (p n : Int32)
-  (hppos : 0 < p) (hnpos : 0 < n)
+theorem mark_sieve_marked_of_marked {L : ℕ} (S : Sieve L) (n : Int32)
+  (hnpos : 0 < n)
   (nlt : n.toInt.natAbs < S.divs.size)
-  (hprime : Nat.Prime p.toInt.natAbs)
-  (hnextp : ∀ q, Nat.Prime q → (q : ℤ) < p.toInt →
-    (q : ℤ) ∈ (Array.map Int32.toInt S.primes))
-  (hdvd : p.toInt ∣ n.toInt) :
+  (hdvd : S.p.toInt ∣ n.toInt) :
   ∀ i, (ilt : i < S.divs.size) → S.divs[i]'ilt ≠ 0 →
-  (mark_sieve S p n hppos hnpos nlt hprime hnextp hdvd).divs[i]'(by simpa) ≠ 0 := by
+  (mark_sieve S n hnpos nlt hdvd).divs[i]'(by simpa) ≠ 0 := by
   intro i ilt hmark
   unfold mark_sieve; simp
   split_ifs with h
@@ -175,19 +194,17 @@ theorem mark_sieve_marked_of_marked {L : ℕ} (S : Sieve L) (p n : Int32)
   · exact hmark
 
 -- The given index is non-zero after calling 'mark_sieve'
-theorem mark_sieve_index_marked {L : ℕ} (S : Sieve L) (p n : Int32)
-  (hppos : 0 < p) (hnpos : 0 < n)
+theorem mark_sieve_index_marked {L : ℕ} (S : Sieve L) (n : Int32)
+  (hnpos : 0 < n)
   (nlt : n.toInt.natAbs < S.divs.size)
-  (hprime : Nat.Prime p.toInt.natAbs)
-  (hnextp : ∀ q, Nat.Prime q → (q : ℤ) < p.toInt →
-    (q : ℤ) ∈ (Array.map Int32.toInt S.primes))
-  (hdvd : p.toInt ∣ n.toInt) :
-  (mark_sieve S p n hppos hnpos nlt hprime hnextp hdvd).divs[n.toInt.natAbs]'(by simpa) ≠ 0 := by
+  (hdvd : S.p.toInt ∣ n.toInt) :
+  (mark_sieve S n hnpos nlt hdvd).divs[n.toInt.natAbs]'(by simpa) ≠ 0 := by
   unfold mark_sieve; dsimp
   split_ifs with h
   · rw [Array.getElem_set]; simp
-    contrapose! hppos
-    rw [hppos]; simp
+    intro hpz
+    absurd S.hppos
+    rw [hpz]; simp
   · assumption
 
 lemma int32_toInt_lt_of_lt_divs_size {L : ℕ} (S : Sieve L) (n : Int32)
@@ -216,16 +233,16 @@ lemma int32_toInt_add_of_pos_of_dvd_of_lt (m n : Int32)
     exact (Int.mul_lt_mul_right (two_pos)).mpr hnlt
 
 -- Prove the termination requirements for 'mark_multiple'
-lemma mark_multiple_termination {L : ℕ} (S : Sieve L) (p n : Int32)
-  (hppos : 0 < p) (hnpos : 0 < n)
-  (hdvd : p.toInt ∣ n.toInt)
+lemma mark_multiple_termination {L : ℕ} (S : Sieve L) (n : Int32)
+  (hnpos : 0 < n)
+  (hdvd : S.p.toInt ∣ n.toInt)
   (hnlt : n.toInt.natAbs < S.divs.size) :
-  S.divs.size - (n + p).toInt.natAbs < S.divs.size - n.toInt.natAbs := by
-  have hppos' := int32_toInt_pos_of_pos hppos
+  S.divs.size - (n + S.p).toInt.natAbs < S.divs.size - n.toInt.natAbs := by
+  have hppos' := int32_toInt_pos_of_pos S.hppos
   have hnpos' := int32_toInt_pos_of_pos hnpos
-  have hnp : (n + p).toInt = n.toInt + p.toInt := by
+  have hnp : (n + S.p).toInt = n.toInt + S.p.toInt := by
     rw [Int.add_comm, Int32.add_comm]
-    apply int32_toInt_add_of_pos_of_dvd_of_lt p n hppos hnpos hdvd
+    apply int32_toInt_add_of_pos_of_dvd_of_lt S.p n S.hppos hnpos hdvd
     exact int32_toInt_lt_of_lt_divs_size S _ hnlt
   rw [hnp]
   apply Nat.sub_lt_sub_left hnlt
@@ -233,30 +250,27 @@ lemma mark_multiple_termination {L : ℕ} (S : Sieve L) (p n : Int32)
   exact Int.lt_add_of_pos_right _ hppos'
 
 -- Mark one multiple of 'p' in sieve 'S'
-def mark_multiple {L : ℕ} (S : Sieve L) (p n : Int32)
-  (hppos : 0 < p) (hnpos : 0 < n)
-  (hprime : Nat.Prime p.toInt.natAbs)
-  (hnextp : ∀ q, Nat.Prime q → (q : ℤ) < p.toInt →
-    (q : ℤ) ∈ (Array.map Int32.toInt S.primes))
-  (hdvd : p.toInt ∣ n.toInt) : Sieve L :=
+def mark_multiple {L : ℕ} (S : Sieve L) (n : Int32)
+  (hnpos : 0 < n)
+  (hdvd : S.p.toInt ∣ n.toInt) : Sieve L :=
   if hnlt : n.toInt.natAbs < S.divs.size then
-  (fun (hnp : (n + p).toInt = n.toInt + p.toInt) ↦
+  (fun (hnp : (n + S.p).toInt = n.toInt + S.p.toInt) ↦
     mark_multiple
-      (mark_sieve S p n hppos hnpos hnlt hprime hnextp hdvd)
-      p (n + p) hppos (by
+      (mark_sieve S n hnpos hnlt hdvd)
+      (n + S.p) (by
         apply Int32.lt_iff_toInt_lt.mpr
         rw [hnp]
         apply Int.add_pos (Int32.lt_iff_toInt_lt.mp hnpos)
-        exact Int32.lt_iff_toInt_lt.mp hppos
-      ) hprime hnextp (by
+        exact Int32.lt_iff_toInt_lt.mp S.hppos
+      ) (by
         rw [hnp]
         exact Int.dvd_add hdvd (by use 1; simp)
       ))
   (by
-    have hppos' := int32_toInt_pos_of_pos hppos
+    have hppos' := int32_toInt_pos_of_pos S.hppos
     have hnpos' := int32_toInt_pos_of_pos hnpos
     rw [Int.add_comm, Int32.add_comm]
-    apply int32_toInt_add_of_pos_of_dvd_of_lt p n hppos hnpos hdvd
+    apply int32_toInt_add_of_pos_of_dvd_of_lt S.p n S.hppos hnpos hdvd
     exact int32_toInt_lt_of_lt_divs_size S _ hnlt
   ) else S
 termination_by S.divs.size - n.toInt.natAbs
@@ -265,30 +279,20 @@ decreasing_by
   apply mark_multiple_termination <;> assumption
 
 -- Mark all multiples of the next prime, 'p', in the Sieve
-def mark_multiples {L : ℕ} (S : Sieve L) (p : Int32)
-  (hppos : 0 < p)
-  (hprime : Nat.Prime p.toInt.natAbs)
-  (hnextp : ∀ q, Nat.Prime q → (q : ℤ) < p.toInt →
-    (q : ℤ) ∈ (Array.map Int32.toInt S.primes)) : Sieve L :=
-  mark_multiple S p p hppos hppos hprime hnextp (by use 1; simp)
+def mark_multiples {L : ℕ} (S : Sieve L) : Sieve L :=
+  mark_multiple S S.p S.hppos (by use 1; simp)
 
-@[simp] theorem mark_multiple_divs_size {L : ℕ} (S : Sieve L) (p n : Int32)
-  (hppos : 0 < p) (hnpos : 0 < n)
-  (hprime : Nat.Prime p.toInt.natAbs)
-  (hnextp : ∀ q, Nat.Prime q → (q : ℤ) < p.toInt →
-    (q : ℤ) ∈ (Array.map Int32.toInt S.primes))
-  (hdvd : p.toInt ∣ n.toInt) :
-  (mark_multiple S p n hppos hnpos hprime hnextp hdvd).divs.size = S.divs.size := by
+@[simp] theorem mark_multiple_divs_size {L : ℕ} (S : Sieve L) (n : Int32)
+  (hnpos : 0 < n)
+  (hdvd : S.p.toInt ∣ n.toInt) :
+  (mark_multiple S n hnpos hdvd).divs.size = S.divs.size := by
   rw [Sieve.hsize, Sieve.hsize]
 
 -- The 'primes' field is unchanged by 'mark_multiple'
-@[simp] theorem mark_multiple_primes {L : ℕ} (S : Sieve L) (p n : Int32)
-  (hppos : 0 < p) (hnpos : 0 < n)
-  (hprime : Nat.Prime p.toInt.natAbs)
-  (hnextp : ∀ q, Nat.Prime q → (q : ℤ) < p.toInt →
-    (q : ℤ) ∈ (Array.map Int32.toInt S.primes))
-  (hdvd : p.toInt ∣ n.toInt) :
-  (mark_multiple S p n hppos hnpos hprime hnextp hdvd).primes = S.primes := by
+@[simp] theorem mark_multiple_primes {L : ℕ} (S : Sieve L) (n : Int32)
+  (hnpos : 0 < n)
+  (hdvd : S.p.toInt ∣ n.toInt) :
+  (mark_multiple S n hnpos hdvd).primes = S.primes := by
   unfold mark_multiple; simp
   split_ifs with h
   · apply mark_multiple_primes
@@ -299,14 +303,11 @@ decreasing_by
   apply mark_multiple_termination <;> assumption
 
 -- Every cell marked in 'S' is also marked in 'mark_multiple S'
-theorem mark_multiple_marked_of_marked {L : ℕ} (S : Sieve L) (p n : Int32)
-  (hppos : 0 < p) (hnpos : 0 < n)
-  (hprime : Nat.Prime p.toInt.natAbs)
-  (hnextp : ∀ q, Nat.Prime q → (q : ℤ) < p.toInt →
-    (q : ℤ) ∈ (Array.map Int32.toInt S.primes))
-  (hdvd : p.toInt ∣ n.toInt) :
+theorem mark_multiple_marked_of_marked {L : ℕ} (S : Sieve L) (n : Int32)
+  (hnpos : 0 < n)
+  (hdvd : S.p.toInt ∣ n.toInt) :
   ∀ i, (ilt : i < S.divs.size) → S.divs[i]'ilt ≠ 0 →
-  (mark_multiple S p n hppos hnpos hprime hnextp hdvd).divs[i]'(by simpa) ≠ 0 := by
+  (mark_multiple S n hnpos hdvd).divs[i]'(by simpa) ≠ 0 := by
   intro i ilt hmark
   unfold mark_multiple; dsimp
   split_ifs with h
@@ -321,18 +322,15 @@ decreasing_by
 
 -- Show that 'mark_multiple' does indeed mark every
 -- multiple of 'p' greater than or equal to 'n'
-theorem mark_multiple_verify {L : ℕ} (S : Sieve L) (p n : Int32)
-  (hppos : 0 < p) (hnpos : 0 < n)
-  (hprime : Nat.Prime p.toInt.natAbs)
-  (hnextp : ∀ q, Nat.Prime q → (q : ℤ) < p.toInt →
-    (q : ℤ) ∈ (Array.map Int32.toInt S.primes))
-  (hdvd : p.toInt ∣ n.toInt) :
+theorem mark_multiple_verify {L : ℕ} (S : Sieve L) (n : Int32)
+  (hnpos : 0 < n)
+  (hdvd : S.p.toInt ∣ n.toInt) :
   ∀ (i : ℕ), (n.toInt ≤ (i : ℤ)) → (ilt : i < S.divs.size) →
-    p.toInt ∣ (i : ℤ) →
-  (mark_multiple S p n hppos hnpos hprime hnextp hdvd).divs[i]'(by
+    S.p.toInt ∣ (i : ℤ) →
+  (mark_multiple S n hnpos hdvd).divs[i]'(by
     rwa [mark_multiple_divs_size]
   ) ≠ 0 := by
-  have hppos' := int32_toInt_pos_of_pos hppos
+  have hppos' := int32_toInt_pos_of_pos S.hppos
   have hnpos' := int32_toInt_pos_of_pos hnpos
   have hnabs : (n.toInt.natAbs : ℤ) = n.toInt := Int.natAbs_of_nonneg (le_of_lt hnpos')
   intro i nlei ilt pdvdi
@@ -343,26 +341,25 @@ theorem mark_multiple_verify {L : ℕ} (S : Sieve L) (p n : Int32)
       int32_toInt_lt_of_lt_divs_size S _ h
     have ipos : 0 < (i : ℤ) :=
       lt_of_lt_of_le (int32_toInt_pos_of_pos hnpos) nlei
-    have := int32_toInt_add_of_pos_of_dvd_of_lt p n hppos hnpos hdvd hnlt
+    have := int32_toInt_add_of_pos_of_dvd_of_lt S.p n S.hppos hnpos hdvd hnlt
     rw [Int.add_comm, Int32.add_comm] at this
-    have hnppos : 0 < n + p := by
+    have hnppos : 0 < n + S.p := by
       apply Int32.lt_iff_toInt_lt.mpr
       rw [this]; simp
       exact Int.add_pos hnpos' hppos'
-    have hdvd' : p.toInt ∣ (n + p).toInt := by
+    have hdvd' : S.p.toInt ∣ (n + S.p).toInt := by
       rw [this]
       exact Int.dvd_add hdvd (by use 1; simp)
-    let S' := (mark_sieve S p n hppos hnpos h hprime hnextp hdvd)
+    let S' := (mark_sieve S n hnpos h hdvd)
     have hnextp' :
-      ∀ (q : ℕ), Nat.Prime q → ↑q < p.toInt → ↑q ∈ Array.map Int32.toInt S'.primes := by
+      ∀ (q : ℕ), Nat.Prime q → ↑q < S.p.toInt → ↑q ∈ Array.map Int32.toInt S'.primes := by
       intro q qprime qlt
       unfold S'
       rw [mark_sieve_primes]
-      exact hnextp q qprime qlt
-    by_cases hnple : (n + p).toInt ≤ (i : ℤ)
-    · apply mark_multiple_verify S' p (n + p) hppos hnppos hprime hnextp' hdvd' i hnple _ pdvdi
-      unfold S'
-      rwa [mark_sieve_divs_size]
+      exact S.hpnext q qprime qlt
+    by_cases hnple : (n + S.p).toInt ≤ (i : ℤ)
+    · apply mark_multiple_verify S' (n + S.p) hnppos hdvd' i hnple _ pdvdi
+      unfold S'; simpa
     rename' hnple => ilt'; push_neg at ilt'
     -- At this point, from nlei, ilt', and pdvdi we can conclude that i = n
     rw [this] at ilt'
@@ -371,7 +368,7 @@ theorem mark_multiple_verify {L : ℕ} (S : Sieve L) (p n : Int32)
     rcases hdvdcp with ⟨kn, hnpk⟩
     rw [hipk, hnpk] at ilt'
     rw [hipk, hnpk] at nlei
-    nth_rw 3 [← Int.mul_one p.toInt] at ilt'
+    nth_rw 3 [← Int.mul_one S.p.toInt] at ilt'
     rw [← Int.mul_add] at ilt'
     apply (Int.mul_lt_mul_left hppos').mp at ilt'
     apply (Int.mul_le_mul_left hppos').mp at nlei
@@ -379,7 +376,7 @@ theorem mark_multiple_verify {L : ℕ} (S : Sieve L) (p n : Int32)
     rw [← hknki, ← hnpk] at hipk
     rename' hipk => hin
     apply mark_multiple_marked_of_marked
-    · convert mark_sieve_index_marked S p n hppos hnpos h hprime hnextp hdvd
+    · convert mark_sieve_index_marked S n hnpos h hdvd
       apply Int.ofNat_inj.mp; symm
       exact hin ▸ hnabs
     simpa
@@ -394,14 +391,10 @@ decreasing_by
   apply mark_multiple_termination <;> assumption
 
 -- Verify that 'mark_multiples' does indeed mark every multiple of 'p'
-theorem mark_multiples_verify (S : Sieve L) (p : Int32)
-  (hppos : 0 < p)
-  (hprime : Nat.Prime p.toInt.natAbs)
-  (hnextp : ∀ q, Nat.Prime q → (q : ℤ) < p.toInt →
-    (q : ℤ) ∈ (Array.map Int32.toInt S.primes)) :
+theorem mark_multiples_verify {L : ℕ} (S : Sieve L) :
   ∀ (i : ℕ), (0 < i) → (ilt : i < S.divs.size) →
-    p.toInt ∣ (i : ℤ) →
-  (mark_multiples S p hppos hprime hnextp).divs[i]'(by
+    S.p.toInt ∣ (i : ℤ) →
+  (mark_multiples S).divs[i]'(by
     unfold mark_multiples; simpa
   ) ≠ 0 := by
   intro i hipos ilt pdvdi
